\documentclass{article} 
\usepackage{amsmath}
\usepackage{graphicx}
\usepackage[a4paper, left=1.5in, right=1.5in, top=1.5in, bottom=1.5in]{geometry}
\usepackage{xcolor}

\begin{document}

\title{calculus is a branch of mathematics that deals with rates of change and the accumulation of quantities.}

\maketitle


circle: $(x-a)^2 + (y-b)^2 = r^2$ where $(a, b)$ is the center and the radius is $r$\\

midpoint between $P_1 = (x_1, y_1)$ and $P_2 = (x_2, y_2)$ is $\bar{P_{1}P_2}$ divided by 2\\

distance: $\sqrt{(x_2 - x_1)^2 + (y_2 - y_1)^2}$\\

laws of exponents: 

	\begin{itemize}
		\item $x^mx^n = x^{m+n}$
		\item $\frac{x^m}{x^n} = x^{m-n}$
		\item $(x^m)^n = x^{mn}$
		\item $x^{-n} = \frac{1}{x^n}$
		\item $(xy)^n = x^ny^n$
		\item $(\frac{x}{y})^n = \frac{x^n}{y^n}$
		\item $x^{1/n} = \sqrt[n]{x}$
		\item $x^{\frac{m}{n}} = \sqrt[n]{x^m} = (\sqrt[n]{x})^m$
	\end{itemize}

special factorizations

	\begin{itemize}
		\item $x^2 - y^2 = (x + y)(x - y)$
		\item $x^3 + y^3 = (x + y)(x^2 - xy + y^2)$
		\item $x^3 - y^3 = (x - y)(x^2 + xy + y^2)$
	\end{itemize}

binomial theorem:

	\begin{itemize}
		\item $(x + y)^2 = x^2 + 2xy + y^2$
		\item $(x - y)^2 = x^2 - 2xy + y^2$
		\item $(x + y)^3 = x^3 + 3x^2y + 3xy^2 + y^3$
		\item $(x - y)^3 = x^3 - 3x^2y + 3xy^2 - y^3$
		\item $(x + y)^n = x^n + nx^{n-1}y + \frac{n(n-1)}{2}x^{n-2}y^2 + \ldots + \binom{n}{k}x^{n-k}y^k + \dots + nxy^{n-1} + y^n$
			where $\binom{n}{k} = \frac{n(n-1) \dots (n-k+1)}{1 \cdot 2 \cdot 3 \cdot \ldots \cdot k}$
	\end{itemize}

quadratic formulae:

	\begin{enumerate}
		\item $ax^2 + bx + c = 0$
		\item $x^2 + \frac{b}{a}x + \frac{c}{a} = 0$
		\item $x^2 + \frac{b}{a}x = -\frac{c}{a}$
		\item $x^2 + \frac{b}{a}x + \left( \frac{b}{2a} \right)^2 = -\frac{c}{a} + \left( \frac{b}{2a} \right)^2$
		\item $\left( x + \frac{b}{2a} \right)^2 = \frac{b^2 - 4ac}{4a^2}$
		\item $x + \frac{b}{2a} = \pm \frac{\sqrt{b^2 - 4ac}}{2a}$
		\item $x = -\frac{b}{2a} \pm \frac{\sqrt{b^2 - 4ac}}{2a}$
		\item $x = \frac{-b \pm \sqrt{b^2 - 4ac}}{2a}$
	\end{enumerate}

polynomials $a_nx^n + a_{n-1}x^{n-1} + ... + a_1x + a_0$ where n is non-neg and represents the degree\\

rational $p(x)/q(x)$\\

root $\sqrt[n]{g(x)}$\\

properties:\\
	domain: set of all input values for which the function is defined\\
	range: set of all possible output values of the function\\
	
	continuity: most algebaic functions are continuous (no breaks of jumps), but rational functions have discontinuities at points\\
		
	behavior: the functions behavior is influenced bu the degree of the polynomial and the nature of the function\\


	scaling:\\
		\begin{itemize}
			\item{vertical scaling} $y = kf(x)$: If $k \geq 1$, the graph is expanded vertically by the factor $k$. If $0 < k < 1$, the graph is compressed vertically. When the scale factor $k$ is negative $(k < 0)$, the graph is also reflected across the x-axis.
			\item{horizontal scaling} $y = f(kx)$: If $K \geq 1$, the graph is compressed in the horizontal direction. If $0 < k < 1$, the graph is expanded. If $k \leq 0$, then the graph is also reflected across the y-axis.
		\end{itemize}

$1 \deg = \frac{\pi}{180}$rad\\

trigonometric functions are mathematical functions that relate the angle of a trianlge to the lengths of its sides. these functions are based on the relationships between the angles and sides of right-angled triangles and can also be generalized to all real numbers using the unit circle.\\

To derive the rest of the fundamental trigonometric identities, you need a combination of a few key identities and principles. The most important starting point is the Pythagorean identity, but youâ€™ll also need the basic relationships between the trigonometric functions, such as the definitions of sine, cosine, tangent, secant, cosecant, and cotangent in terms of a right triangle or the unit circle. \\

$ \sin^2 \theta + \cos^2 \theta = 1 $\\

$ \sec \theta = \frac{1}{\cos \theta}, \quad \csc \theta = \frac{1}{\sin \theta}, \quad \cot \theta = \frac{1}{\tan \theta} $\\

$ \tan \theta = \frac{\sin \theta}{\cos \theta}, \quad \cot \theta = \frac{\cos \theta}{\sin \theta} $\\

$ 1 + \tan^2 \theta = \sec^2 \theta $\\

$ 1 + \cot^2 \theta = \csc^2 \theta $\\

$ \sin(\alpha + \beta) = \sin \alpha \cos \beta + \cos \alpha \sin \beta $\\

$ \cos(\alpha + \beta) = \cos \alpha \cos \beta - \sin \alpha \sin \beta $\\

$ \tan(\alpha + \beta) = \frac{\tan \alpha + \tan \beta}{1 - \tan \alpha \tan \beta} $\\

$ \sin(\alpha - \beta) = \sin \alpha \cos \beta - \cos \alpha \sin \beta $\\

$ \cos(\alpha - \beta) = \cos \alpha \cos \beta + \sin \alpha \sin \beta $\\

$ \tan(\alpha - \beta) = \frac{\tan \alpha - \tan \beta}{1 + \tan \alpha \tan \beta} $\\

$ \sin(2\theta) = 2\sin \theta \cos \theta $\\

$ \cos(2\theta) = \cos^2 \theta - \sin^2 \theta = 2\cos^2 \theta - 1 = 1 - 2\sin^2 \theta $\\

$ \tan(2\theta) = \frac{2\tan \theta}{1 - \tan^2 \theta} $\\

$ \sin(90^\circ - \theta) = \cos \theta, \quad \cos(90^\circ - \theta) = \sin \theta $\\

$ \tan(90^\circ - \theta) = \cot \theta, \quad \cot(90^\circ - \theta) = \tan \theta $\\

$ \sec(90^\circ - \theta) = \csc \theta, \quad \csc(90^\circ - \theta) = \sec \theta $\\

$ \sin(-\theta) = -\sin(\theta), \quad \cos(-\theta) = \cos(\theta) $\\

$ \tan(-\theta) = -\tan(\theta), \quad \sec(-\theta) = \sec(\theta) $\\

$ \csc(-\theta) = -\csc(\theta), \quad \cot(-\theta) = -\cot(\theta) $\\

$ \sin \alpha \sin \beta = \frac{1}{2} [\cos(\alpha - \beta) - \cos(\alpha + \beta)] $\\

$ \cos \alpha \cos \beta = \frac{1}{2} [\cos(\alpha - \beta) + \cos(\alpha + \beta)] $\\

$ \sin \alpha \cos \beta = \frac{1}{2} [\sin(\alpha + \beta) + \sin(\alpha - \beta)] $\\

power functions: $f(x) = x^n$....if even the function behaves symmetrical around the y-axis...if odd then the function has point symmetry ($x^4$, $x^3$, $x^{-n} = \frac{1}{x^n}$)\\

inverse trig functions: $\arcsin(x) = \sin^{-1}(x) = \theta$, $\arccos(x) = \cos^{-1}(x) = \theta$, $\arcsin(x) = \sin^{-1}(x) = \theta$\\

logs: $\log_ax=y \leftrightarrow a^y = x$, $\ln(x)=y \leftrightarrow e^y=x$\\

hyperbolic functions: $\sinh(x) = \frac{e^x-e^{-x}}{2}$, $\cosh(x) = \frac{e^x+e^{-x}}{2}$, $\tanh(x) = \frac{\sinh(x)}{\cosh(x)}$\\

differentiation rules:
	\begin{enumerate}
		\item$\frac{d}{dx}(c) = 0$
		\item$\frac{d}{dx}x = 1$
		\item$\frac{d}{dx}(x^n) = nx^{-1}$ (power rule)
		\item$\frac{d}{dx}[cf(x)] = cf'(x)$
		\item$\frac{d}{dx}[f(x)+g(x)] = f'(x) + g'(x)$
		\item$\frac{d}{dx}[f(x)g(x)] = f(x)g'(x) + g(x)f'(x)$ (product rule)
		\item$\frac{d}{dx}[\frac{f(x)}{g(x)}] = \frac{g(x)f'(x) - f(x)g'(x)}{[g(x)]^2}$ (quotient rule)
		\item$\frac{d}{dx}$ (chain rule)
		\item$\frac{d}{dx}$ (quotient rule)
		\item$\frac{d}{dx}$ (chain rule)
		\item$\frac{d}{dx}$ (general power rule)
		\item$\frac{d}{dx}$ 
		\item$\frac{d}{dx}$
		\item$\frac{d}{dx}$
		\item$\frac{d}{dx}$
		\item$\frac{d}{dx}$
		\item$\frac{d}{dx}$
		\item$\frac{d}{dx}$
		\item$\frac{d}{dx}$
		\item$\frac{d}{dx}$
		\item$\frac{d}{dx}$
		\item$\frac{d}{dx}$
		\item$\frac{d}{dx}$
		\item$\frac{d}{dx}$
		\item$\frac{d}{dx}$
		\item$\frac{d}{dx}$
		\item$\frac{d}{dx}$
		\item$\frac{d}{dx}$
		\item$\frac{d}{dx}$
		\item$\frac{d}{dx}$	
	\end{enumerate}

\newpage
\section*{problems}	
				
\end{document}























